rupicola/io/ExamplesIO.fst
@@ -7,8 +7,8 @@ let u_return () : io bool = return true
 let apply_io_return : bool -> io bool = fun x -> io_return x
 
 let apply_read () : io (resexn bool) = read 0
-let apply_write_const () : io (resexn unit) = write (2,true)
-let apply_write : bool -> io (resexn unit) = fun x -> write (1,x)
+let apply_write_const () : io (resexn unit) = write (2,"hello")
+let apply_write : string -> io (resexn unit) = fun x -> write (1,x)
 
 let apply_io_bind_const () : io bool =
   let!@ x = io_return true in
@@ -24,24 +24,24 @@ let apply_io_bind_pure_if : bool -> io bool =
     if!@ (io_return x) then io_return false
     else io_return true
 
-let apply_io_bind_write : bool -> io (resexn unit) =
+let apply_io_bind_write : string -> io (resexn unit) =
   fun x ->
     let!@ y = io_return x in
     write (2,y)
 
 let apply_io_bind_read_write () : io (resexn unit) =
   match!@ read 4 with
-  | Inl x -> write (1,x)
+  | Inl _ -> write (1,"data")
   | Inr x -> io_return (Inr x)
 
 let apply_io_bind_read_write' () : io (resexn unit) =
-  io_bind (read 9) (fun x -> match x with | Inl x -> write (2,x) | Inr x -> io_return (Inr x))
+  io_bind (read 9) (fun x -> match x with | Inl _ -> write (2,"data") | Inr x -> io_return (Inr x))
 
 let apply_io_bind_read_if_write () : io (resexn unit) =
   match!@ read 0 with
   | Inl x -> if x
-            then write (7,false)
-            else write (8,true)
+            then write (7,"data")
+            else write (8,"data")
   | Inr x -> return (Inr x)
 
 (** Examples inspired from the Web Server **)
@@ -49,9 +49,7 @@ val utf8_encode : bool -> bool
 let utf8_encode x = x
 
 let sendError400 (fd:bool) : io unit =
-  let x = utf8_encode true in
-  let p = (fd, x) in
-  write (9, fd) ;!@
+  write (9, "error400") ;!@
   return ()
 
 let get_req (fd:bool) : io (either bool bool) =
@@ -68,5 +66,5 @@ let (let!@!) #a #b (m:io (resexn a)) (k:a -> io (resexn b)) =
 let open2_read_write () =
   let!@! fd1 = openfile "/tmp/input" in
   let!@! fd2 = openfile "/tmp/output" in
-  let!@! msg = read fd1 in
-  write (fd2, msg)
+  let!@! _ = read fd1 in
+  write (fd2, "data")
